src/extraction/FStar.Extraction.ML.Modul.fsti
@@ -20,6 +20,12 @@ open FStar.Compiler.Effect
 open FStar.Syntax.Syntax
 open FStar.Extraction.ML.Syntax
 open FStar.Extraction.ML.UEnv
+module S = FStar.Syntax.Syntax
+
+type extension_extractor = 
+   uenv -> FStar.Compiler.Dyn.dyn -> either (mlexpr * e_tag * mlty) string
+
+val register_extension_extractor (extension_name:string) (extractor:extension_extractor) : unit
 
 val iface : Type0
 val extract_iface: uenv -> modul -> uenv * iface
