src/syntax/FStar.Syntax.Print.fst
@@ -163,7 +163,7 @@ let paren s = "(" ^ s ^ ")"
    redexes that should first be reduced. *)
 let rec tag_of_term (t:term) = match t.n with
   | Tm_bvar x -> "Tm_bvar: "   ^ db_to_string x
-  | Tm_name x -> "Tm_name: " ^ nm_to_string x
+  | Tm_name x -> "Tm_name: " ^ nm_to_string x ^ "@" ^ (tag_of_term x.sort)
   | Tm_fvar x -> "Tm_fvar: "   ^ lid_to_string x.fv_name.v
   | Tm_uinst _ -> "Tm_uinst"
   | Tm_constant _ -> "Tm_constant"
